case_study/RiscvPmp/Base.v
@@ -45,245 +45,226 @@ Definition Xlenbits : Set := Z.
 Definition Addr : Set := Z.
 Definition Word : Set := Z.
 
-Module Enums.
-  Inductive Privilege : Set :=
-  | User
-  | Machine
-  .
+Inductive Privilege : Set :=
+| User
+| Machine
+.
 
-  (* Ignore execute perm for now *)
-  Inductive Permission : Set :=
-  | O
-  | R
-  | W
-  | RW.
+(* Enum for available CRSs' *)
+Inductive CSRIdx : Set :=
+| MStatus
+| MTvec
+| MCause
+| MEpc
+.
 
+(* NOTE: PMP CSRs limited to 1 for now *)
+Inductive PmpCfgIdx : Set :=
+| PMP0CFG
+| PMP1CFG
+.
 
-  (* Enum for available CRSs' *)
-  Inductive CSRIdx : Set :=
-  | MStatus
-  | MTvec
-  | MCause
-  | MEpc
-  .
+Inductive PmpAddrIdx : Set :=
+| PMPADDR0
+| PMPADDR1
+.
 
-  (* NOTE: PMP CSRs limited to 1 for now *)
-  Inductive PmpCfgIdx : Set :=
-  | PMP0CFG
-  | PMP1CFG
-  .
+(* NOTE: PMP Addr Match Type limited to OFF and TOR for now *)
+Inductive PmpAddrMatchType : Set :=
+| OFF
+| TOR
+.
 
-  Inductive PmpAddrIdx : Set :=
-  | PMPADDR0
-  | PMPADDR1
-  .
+Inductive PmpMatch : Set :=
+| PMP_Success
+| PMP_Continue
+| PMP_Fail
+.
 
-  (* NOTE: PMP Addr Match Type limited to OFF and TOR for now *)
-  Inductive PmpAddrMatchType : Set :=
-  | OFF
-  | TOR
-  .
+Inductive PmpAddrMatch : Set :=
+| PMP_NoMatch
+| PMP_PartialMatch
+| PMP_Match
+.
 
-  Inductive PmpMatch : Set :=
-  | PMP_Success
-  | PMP_Continue
-  | PMP_Fail
-  .
+Inductive ROP : Set :=
+| RISCV_ADD
+| RISCV_SUB
+.
 
-  Inductive PmpAddrMatch : Set :=
-  | PMP_NoMatch
-  | PMP_PartialMatch
-  | PMP_Match
-  .
+Inductive IOP : Set :=
+| RISCV_ADDI
+.
 
-  Inductive ROP : Set :=
-  | RISCV_ADD
-  | RISCV_SUB
-  .
+Inductive UOP : Set :=
+| RISCV_LUI
+| RISCV_AUIPC
+.
 
-  Inductive IOP : Set :=
-  | RISCV_ADDI
-  .
+Inductive BOP : Set :=
+| RISCV_BEQ
+| RISCV_BNE
+| RISCV_BLT
+| RISCV_BGE
+| RISCV_BLTU
+| RISCV_BGEU
+.
 
-  Inductive UOP : Set :=
-  | RISCV_LUI
-  | RISCV_AUIPC
-  .
+(* Zicsr extension, only support for Read-Write (no set or clear) *)
+Inductive CSROP : Set :=
+| CSRRW
+.
 
-  Inductive BOP : Set :=
-  | RISCV_BEQ
-  | RISCV_BNE
-  | RISCV_BLT
-  | RISCV_BGE
-  | RISCV_BLTU
-  | RISCV_BGEU
-  .
+Inductive Retired : Set :=
+| RETIRE_SUCCESS
+| RETIRE_FAIL.
 
-  (* Zicsr extension, only support for Read-Write (no set or clear) *)
-  Inductive CSROP : Set :=
-  | CSRRW
-  .
+Inductive Enums : Set :=
+| privilege
+| csridx
+| pmpcfgidx
+| pmpaddridx
+| pmpaddrmatchtype
+| pmpmatch
+| pmpaddrmatch
+| rop
+| iop
+| uop
+| bop
+| csrop
+| retired
+.
 
-  Inductive Retired : Set :=
-  | RETIRE_SUCCESS
-  | RETIRE_FAIL.
+Definition RegIdx := bv 3.
+Bind Scope bv_scope with RegIdx.
 
-  Inductive Enums : Set :=
-  | privilege
-  | permission
-  | csridx
-  | pmpcfgidx
-  | pmpaddridx
-  | pmpaddrmatchtype
-  | pmpmatch
-  | pmpaddrmatch
-  | rop
-  | iop
-  | uop
-  | bop
-  | csrop
-  | retired
-  .
-End Enums.
-Import Enums.
+Inductive AST : Set :=
+| RTYPE (rs2 rs1 rd : RegIdx) (op : ROP)
+| ITYPE (imm : Z) (rs1 rd : RegIdx) (op : IOP)
+| UTYPE (imm : Z) (rd : RegIdx) (op : UOP)
+| BTYPE (imm : Z) (rs2 rs1 : RegIdx) (op : BOP)
+| RISCV_JAL (imm : Z) (rd : RegIdx)
+| RISCV_JALR (imm : Z) (rs1 rd : RegIdx)
+| LOAD (imm : Z) (rs1 rd : RegIdx)
+| STORE (imm : Z) (rs2 rs1 : RegIdx)
+| ECALL
+| MRET
+(* Ziscr extension, excluding immediate variants *)
+| CSR (csr : CSRIdx) (rs1 rd : RegIdx) (csrop : CSROP)
+.
 
-Module Unions.
-  Definition RegIdx := bv 3.
-  Bind Scope bv_scope with RegIdx.
+Inductive AccessType : Set :=
+| Read
+| Write
+| ReadWrite
+| Execute
+.
 
-  Inductive AST : Set :=
-  | RTYPE (rs2 rs1 rd : RegIdx) (op : ROP)
-  | ITYPE (imm : Z) (rs1 rd : RegIdx) (op : IOP)
-  | UTYPE (imm : Z) (rd : RegIdx) (op : UOP)
-  | BTYPE (imm : Z) (rs2 rs1 : RegIdx) (op : BOP)
-  | RISCV_JAL (imm : Z) (rd : RegIdx)
-  | RISCV_JALR (imm : Z) (rs1 rd : RegIdx)
-  | LOAD (imm : Z) (rs1 rd : RegIdx)
-  | STORE (imm : Z) (rs2 rs1 : RegIdx)
-  | ECALL
-  | MRET
-  (* Ziscr extension, excluding immediate variants *)
-  | CSR (csr : CSRIdx) (rs1 rd : RegIdx) (csrop : CSROP)
-  .
+Inductive ExceptionType : Set :=
+| E_Fetch_Access_Fault
+| E_Load_Access_Fault
+| E_SAMO_Access_Fault
+| E_U_EnvCall
+| E_M_EnvCall
+| E_Illegal_Instr
+.
 
-  Inductive AccessType : Set :=
-  | Read
-  | Write
-  | ReadWrite
-  | Execute
-  .
+Inductive MemoryOpResult : Set :=
+| MemValue (v : Word)
+| MemException (e : ExceptionType)
+.
 
-  Inductive ExceptionType : Set :=
-  | E_Fetch_Access_Fault
-  | E_Load_Access_Fault
-  | E_SAMO_Access_Fault
-  | E_U_EnvCall
-  | E_M_EnvCall
-  | E_Illegal_Instr
-  .
+Inductive FetchResult : Set :=
+| F_Base (v : Word)
+| F_Error (e : ExceptionType) (v : Xlenbits)
+.
 
-  Inductive MemoryOpResult : Set :=
-  | MemValue (v : Word)
-  | MemException (e : ExceptionType)
-  .
-
-  Inductive FetchResult : Set :=
-  | F_Base (v : Word)
-  | F_Error (e : ExceptionType) (v : Xlenbits)
-  .
-
-  (* NOTE: simplified to only take the ctl_trap constructor into account
+(* NOTE: simplified to only take the ctl_trap constructor into account
          (other constructors are for mret, sret and uret, not considered atm) *)
-  Inductive CtlResult : Set :=
-  | CTL_TRAP (e : ExceptionType)
-  | CTL_MRET
-  .
+Inductive CtlResult : Set :=
+| CTL_TRAP (e : ExceptionType)
+| CTL_MRET
+.
 
-  Inductive ASTConstructor : Set :=
-  | KRTYPE
-  | KITYPE
-  | KUTYPE
-  | KBTYPE
-  | KRISCV_JAL
-  | KRISCV_JALR
-  | KLOAD
-  | KSTORE
-  | KECALL
-  | KMRET
-  | KCSR
-  .
+Inductive ASTConstructor : Set :=
+| KRTYPE
+| KITYPE
+| KUTYPE
+| KBTYPE
+| KRISCV_JAL
+| KRISCV_JALR
+| KLOAD
+| KSTORE
+| KECALL
+| KMRET
+| KCSR
+.
 
-  Inductive AccessTypeConstructor : Set :=
-  | KRead
-  | KWrite
-  | KReadWrite
-  | KExecute
-  .
+Inductive AccessTypeConstructor : Set :=
+| KRead
+| KWrite
+| KReadWrite
+| KExecute
+.
 
-  Inductive ExceptionTypeConstructor : Set :=
-  | KE_Fetch_Access_Fault
-  | KE_Load_Access_Fault
-  | KE_SAMO_Access_Fault
-  | KE_U_EnvCall
-  | KE_M_EnvCall
-  | KE_Illegal_Instr
-  .
+Inductive ExceptionTypeConstructor : Set :=
+| KE_Fetch_Access_Fault
+| KE_Load_Access_Fault
+| KE_SAMO_Access_Fault
+| KE_U_EnvCall
+| KE_M_EnvCall
+| KE_Illegal_Instr
+.
 
-  Inductive MemoryOpResultConstructor : Set :=
-  | KMemValue
-  | KMemException
-  .
+Inductive MemoryOpResultConstructor : Set :=
+| KMemValue
+| KMemException
+.
 
-  Inductive FetchResultConstructor : Set :=
-  | KF_Base
-  | KF_Error
-  .
+Inductive FetchResultConstructor : Set :=
+| KF_Base
+| KF_Error
+.
 
-  Inductive CtlResultConstructor : Set :=
-  | KCTL_TRAP
-  | KCTL_MRET
-  .
+Inductive CtlResultConstructor : Set :=
+| KCTL_TRAP
+| KCTL_MRET
+.
 
-  Inductive Unions : Set :=
-  | ast
-  | access_type
-  | exception_type
-  | memory_op_result
-  | fetch_result
-  | ctl_result
-  (* | pmp_entries *)
-  .
-End Unions.
-Import Unions.
+Inductive Unions : Set :=
+| ast
+| access_type
+| exception_type
+| memory_op_result
+| fetch_result
+| ctl_result
+(* | pmp_entries *)
+.
 
-Module Records.
-  Record Pmpcfg_ent : Set :=
-    MkPmpcfg_ent
-      { L : bool;
-        A : PmpAddrMatchType;
-        X : bool;
-        W : bool;
-        R : bool;
-      }.
+Record Pmpcfg_ent : Set :=
+  MkPmpcfg_ent
+    { L : bool;
+      A : PmpAddrMatchType;
+      X : bool;
+      W : bool;
+      R : bool;
+    }.
 
-  Record Mstatus : Set :=
-    MkMstatus
-      { MPP : Privilege
-      }.
+Record Mstatus : Set :=
+  MkMstatus
+    { MPP : Privilege
+    }.
 
-  Inductive Records : Set :=
-  | rpmpcfg_ent
-  | rmstatus
-  .
-End Records.
-Import Records.
+Inductive Records : Set :=
+| rpmpcfg_ent
+| rmstatus
+.
 
 Section TransparentObligations.
   Local Set Transparent Obligations.
 
   Derive NoConfusion for Enums.
   Derive NoConfusion for Privilege.
-  Derive NoConfusion for Permission.
   Derive NoConfusion for CSRIdx.
   Derive NoConfusion for PmpCfgIdx.
   Derive NoConfusion for PmpAddrIdx.
@@ -316,7 +297,6 @@ End TransparentObligations.
 
 Derive EqDec for Enums.
 Derive EqDec for Privilege.
-Derive EqDec for Permission.
 Derive EqDec for CSRIdx.
 Derive EqDec for PmpCfgIdx.
 Derive EqDec for PmpAddrIdx.
@@ -354,9 +334,6 @@ Section Finite.
 
   Global Program Instance Privilege_finite : Finite Privilege :=
     {| enum := [User;Machine] |}.
-
-  Global Program Instance Permission_finite : Finite Permission :=
-    {| enum := [O;Enums.R;Enums.W;RW] |}.
 
   Global Program Instance CSRIdx_finite : Finite CSRIdx :=
     {| enum := [MStatus;MTvec;MCause;MEpc] |}.
@@ -429,379 +406,377 @@ End Finite.
 
 Module Export RiscvPmpBase <: Base.
 
-Import ctx.notations.
-Import ctx.resolution.
-Import env.notations.
-Import stdpp.finite.
+  Import ctx.notations.
+  Import ctx.resolution.
+  Import env.notations.
+  Import stdpp.finite.
 
-Include DefaultVarKit.
+  Include DefaultVarKit.
 
-Section TypeDeclKit.
+  Section TypeDeclKit.
 
-  (** Enums **)
-  Definition 𝑬        := Enums.
-  Definition 𝑬_eq_dec := Enums_eqdec.
-  Definition 𝑬𝑲 (e : 𝑬) : Set :=
-    match e with
-    | privilege        => Privilege
-    | permission       => Permission
-    | csridx           => CSRIdx
-    | pmpcfgidx        => PmpCfgIdx
-    | pmpaddridx       => PmpAddrIdx
-    | pmpaddrmatchtype => PmpAddrMatchType
-    | pmpmatch         => PmpMatch
-    | pmpaddrmatch     => PmpAddrMatch
-    | rop              => ROP
-    | iop              => IOP
-    | uop              => UOP
-    | bop              => BOP
-    | csrop            => CSROP
-    | retired          => Retired
-    end.
-  Instance 𝑬𝑲_eq_dec (E : 𝑬) : EqDec (𝑬𝑲 E) :=
-    ltac:(destruct E; auto with typeclass_instances).
-  Instance 𝑬𝑲_finite (E : 𝑬) : Finite (𝑬𝑲 E) :=
-    ltac:(destruct E; auto with typeclass_instances).
+    (** Enums **)
+    Definition 𝑬        := Enums.
+    Definition 𝑬_eq_dec := Enums_eqdec.
+    Definition 𝑬𝑲 (e : 𝑬) : Set :=
+      match e with
+      | privilege        => Privilege
+      | csridx           => CSRIdx
+      | pmpcfgidx        => PmpCfgIdx
+      | pmpaddridx       => PmpAddrIdx
+      | pmpaddrmatchtype => PmpAddrMatchType
+      | pmpmatch         => PmpMatch
+      | pmpaddrmatch     => PmpAddrMatch
+      | rop              => ROP
+      | iop              => IOP
+      | uop              => UOP
+      | bop              => BOP
+      | csrop            => CSROP
+      | retired          => Retired
+      end.
+    Instance 𝑬𝑲_eq_dec (E : 𝑬) : EqDec (𝑬𝑲 E) :=
+      ltac:(destruct E; auto with typeclass_instances).
+    Instance 𝑬𝑲_finite (E : 𝑬) : Finite (𝑬𝑲 E) :=
+      ltac:(destruct E; auto with typeclass_instances).
 
-  (** Unions **)
-  Definition 𝑼        := Unions.
-  Definition 𝑼_eq_dec := Unions_eqdec.
-  Definition 𝑼𝑻 (U : 𝑼) : Set :=
-    match U with
-    | ast              => AST
-    | access_type      => AccessType
-    | exception_type   => ExceptionType
-    | memory_op_result => MemoryOpResult
-    | fetch_result     => FetchResult
-    | ctl_result       => CtlResult
-    (* | pmp_entries      => Coq type in the model for pmp_entries  *)
-    end.
-  Instance 𝑼𝑻_eq_dec U : EqDec (𝑼𝑻 U) :=
-    ltac:(destruct U; cbn; auto with typeclass_instances).
+    (** Unions **)
+    Definition 𝑼        := Unions.
+    Definition 𝑼_eq_dec := Unions_eqdec.
+    Definition 𝑼𝑻 (U : 𝑼) : Set :=
+      match U with
+      | ast              => AST
+      | access_type      => AccessType
+      | exception_type   => ExceptionType
+      | memory_op_result => MemoryOpResult
+      | fetch_result     => FetchResult
+      | ctl_result       => CtlResult
+                              (* | pmp_entries      => Coq type in the model for pmp_entries  *)
+      end.
+    Instance 𝑼𝑻_eq_dec U : EqDec (𝑼𝑻 U) :=
+      ltac:(destruct U; cbn; auto with typeclass_instances).
 
-  Definition 𝑼𝑲 (U : 𝑼) : Set :=
-    match U with
-    | ast              => ASTConstructor
-    | access_type      => AccessTypeConstructor
-    | exception_type   => ExceptionTypeConstructor
-    | memory_op_result => MemoryOpResultConstructor
-    | fetch_result     => FetchResultConstructor
-    | ctl_result       => CtlResultConstructor
-    (* | pmp_entries   => PmpEntriesConstructor *)
-    end.
-  Instance 𝑼𝑲_eq_dec U : EqDec (𝑼𝑲 U) :=
-    ltac:(destruct U; auto with typeclass_instances).
-  Instance 𝑼𝑲_finite U : Finite (𝑼𝑲 U) :=
-    ltac:(destruct U; auto with typeclass_instances).
+    Definition 𝑼𝑲 (U : 𝑼) : Set :=
+      match U with
+      | ast              => ASTConstructor
+      | access_type      => AccessTypeConstructor
+      | exception_type   => ExceptionTypeConstructor
+      | memory_op_result => MemoryOpResultConstructor
+      | fetch_result     => FetchResultConstructor
+      | ctl_result       => CtlResultConstructor
+                              (* | pmp_entries   => PmpEntriesConstructor *)
+      end.
+    Instance 𝑼𝑲_eq_dec U : EqDec (𝑼𝑲 U) :=
+      ltac:(destruct U; auto with typeclass_instances).
+    Instance 𝑼𝑲_finite U : Finite (𝑼𝑲 U) :=
+      ltac:(destruct U; auto with typeclass_instances).
 
-  (** Records **)
-  Definition 𝑹        := Records.
-  Definition 𝑹_eq_dec := Records_eqdec.
-  Definition 𝑹𝑻 (R : 𝑹) : Set :=
-    match R with
-    | rpmpcfg_ent => Pmpcfg_ent
-    | rmstatus    => Mstatus
-    end.
-  Instance 𝑹𝑻_eq_dec R : EqDec (𝑹𝑻 R) :=
-    ltac:(destruct R; auto with typeclass_instances).
+    (** Records **)
+    Definition 𝑹        := Records.
+    Definition 𝑹_eq_dec := Records_eqdec.
+    Definition 𝑹𝑻 (R : 𝑹) : Set :=
+      match R with
+      | rpmpcfg_ent => Pmpcfg_ent
+      | rmstatus    => Mstatus
+      end.
+    Instance 𝑹𝑻_eq_dec R : EqDec (𝑹𝑻 R) :=
+      ltac:(destruct R; auto with typeclass_instances).
 
-End TypeDeclKit.
+  End TypeDeclKit.
 
-Include TypeDeclMixin.
+  Include TypeDeclMixin.
 
-(* Override notations of bindigns to put the variable x into string_scope. *)
-Notation "x ∷ t" := (MkB x%string t) : ctx_scope.
+  (* Override notations of bindigns to put the variable x into string_scope. *)
+  Notation "x ∷ t" := (MkB x%string t) : ctx_scope.
 
-Notation ty_xlenbits         := (ty_int).
-Notation ty_word             := (ty_int).
-Notation ty_regno            := (ty_bvec 3).
-Notation ty_privilege        := (ty_enum privilege).
-Notation ty_permission       := (ty_enum permission).
-Notation ty_csridx           := (ty_enum csridx).
-Notation ty_pmpcfgidx        := (ty_enum pmpcfgidx).
-Notation ty_pmpaddridx       := (ty_enum pmpaddridx).
-Notation ty_pmpaddrmatchtype := (ty_enum pmpaddrmatchtype).
-Notation ty_pmpmatch         := (ty_enum pmpmatch).
-Notation ty_pmpaddrmatch     := (ty_enum pmpaddrmatch).
-Notation ty_pmp_addr_range   := (ty_option (ty_prod ty_xlenbits ty_xlenbits)).
-Notation ty_rop              := (ty_enum rop).
-Notation ty_iop              := (ty_enum iop).
-Notation ty_uop              := (ty_enum uop).
-Notation ty_bop              := (ty_enum bop).
-Notation ty_csrop            := (ty_enum csrop).
-Notation ty_retired          := (ty_enum retired).
-Notation ty_mcause           := (ty_xlenbits).
-Notation ty_exc_code         := (ty_int).
-Notation ty_ast              := (ty_union ast).
-Notation ty_access_type      := (ty_union access_type).
-Notation ty_exception_type   := (ty_union exception_type).
-Notation ty_memory_op_result := (ty_union memory_op_result).
-Notation ty_fetch_result     := (ty_union fetch_result).
-Notation ty_ctl_result       := (ty_union ctl_result).
-Notation ty_pmpcfg_ent       := (ty_record rpmpcfg_ent).
-Notation ty_mstatus          := (ty_record rmstatus).
-Notation ty_pmpentry         := (ty_prod ty_pmpcfg_ent ty_xlenbits).
+  Notation ty_xlenbits         := (ty_int).
+  Notation ty_word             := (ty_int).
+  Notation ty_regno            := (ty_bvec 3).
+  Notation ty_privilege        := (ty_enum privilege).
+  Notation ty_csridx           := (ty_enum csridx).
+  Notation ty_pmpcfgidx        := (ty_enum pmpcfgidx).
+  Notation ty_pmpaddridx       := (ty_enum pmpaddridx).
+  Notation ty_pmpaddrmatchtype := (ty_enum pmpaddrmatchtype).
+  Notation ty_pmpmatch         := (ty_enum pmpmatch).
+  Notation ty_pmpaddrmatch     := (ty_enum pmpaddrmatch).
+  Notation ty_pmp_addr_range   := (ty_option (ty_prod ty_xlenbits ty_xlenbits)).
+  Notation ty_rop              := (ty_enum rop).
+  Notation ty_iop              := (ty_enum iop).
+  Notation ty_uop              := (ty_enum uop).
+  Notation ty_bop              := (ty_enum bop).
+  Notation ty_csrop            := (ty_enum csrop).
+  Notation ty_retired          := (ty_enum retired).
+  Notation ty_mcause           := (ty_xlenbits).
+  Notation ty_exc_code         := (ty_int).
+  Notation ty_ast              := (ty_union ast).
+  Notation ty_access_type      := (ty_union access_type).
+  Notation ty_exception_type   := (ty_union exception_type).
+  Notation ty_memory_op_result := (ty_union memory_op_result).
+  Notation ty_fetch_result     := (ty_union fetch_result).
+  Notation ty_ctl_result       := (ty_union ctl_result).
+  Notation ty_pmpcfg_ent       := (ty_record rpmpcfg_ent).
+  Notation ty_mstatus          := (ty_record rmstatus).
+  Notation ty_pmpentry         := (ty_prod ty_pmpcfg_ent ty_xlenbits).
 
-Section TypeDefKit.
+  Section TypeDefKit.
 
-  Open Scope string_scope.
+    Open Scope string_scope.
 
-  (** Unions **)
-  Definition 𝑼𝑲_Ty (U : 𝑼) : 𝑼𝑲 U -> Ty :=
-    match U with
-    | ast              => fun K =>
-                            match K with
-                            | KRTYPE      => ty_tuple [ty_regno; ty_regno; ty_regno; ty_rop]
-                            | KITYPE      => ty_tuple [ty_int; ty_regno; ty_regno; ty_iop]
-                            | KUTYPE      => ty_tuple [ty_int; ty_regno; ty_uop]
-                            | KBTYPE      => ty_tuple [ty_int; ty_regno; ty_regno; ty_bop]
-                            | KRISCV_JAL  => ty_tuple [ty_int; ty_regno]
-                            | KRISCV_JALR => ty_tuple [ty_int; ty_regno; ty_regno]
-                            | KLOAD       => ty_tuple [ty_int; ty_regno; ty_regno]
-                            | KSTORE      => ty_tuple [ty_int; ty_regno; ty_regno]
-                            | KECALL      => ty_unit
-                            | KMRET       => ty_unit
-                            | KCSR        => ty_tuple [ty_csridx; ty_regno; ty_regno; ty_csrop]
-                            end
-    | access_type      => fun _ => ty_unit
-    | exception_type   => fun _ => ty_unit
-    | memory_op_result => fun K =>
-                            match K with
-                            | KMemValue     => ty_word
-                            | KMemException => ty_exception_type
-                            end
-    | fetch_result     => fun K =>
-                            match K with
-                            | KF_Base  => ty_word
-                            | KF_Error => ty_prod ty_exception_type ty_word
-                            end
-    | ctl_result       => fun K =>
-                            match K with
-                            | KCTL_TRAP => ty_exception_type
-                            | KCTL_MRET => ty_unit
-                            end
-    end.
+    (** Unions **)
+    Definition 𝑼𝑲_Ty (U : 𝑼) : 𝑼𝑲 U -> Ty :=
+      match U with
+      | ast              => fun K =>
+                              match K with
+                              | KRTYPE      => ty_tuple [ty_regno; ty_regno; ty_regno; ty_rop]
+                              | KITYPE      => ty_tuple [ty_int; ty_regno; ty_regno; ty_iop]
+                              | KUTYPE      => ty_tuple [ty_int; ty_regno; ty_uop]
+                              | KBTYPE      => ty_tuple [ty_int; ty_regno; ty_regno; ty_bop]
+                              | KRISCV_JAL  => ty_tuple [ty_int; ty_regno]
+                              | KRISCV_JALR => ty_tuple [ty_int; ty_regno; ty_regno]
+                              | KLOAD       => ty_tuple [ty_int; ty_regno; ty_regno]
+                              | KSTORE      => ty_tuple [ty_int; ty_regno; ty_regno]
+                              | KECALL      => ty_unit
+                              | KMRET       => ty_unit
+                              | KCSR        => ty_tuple [ty_csridx; ty_regno; ty_regno; ty_csrop]
+                              end
+      | access_type      => fun _ => ty_unit
+      | exception_type   => fun _ => ty_unit
+      | memory_op_result => fun K =>
+                              match K with
+                              | KMemValue     => ty_word
+                              | KMemException => ty_exception_type
+                              end
+      | fetch_result     => fun K =>
+                              match K with
+                              | KF_Base  => ty_word
+                              | KF_Error => ty_prod ty_exception_type ty_word
+                              end
+      | ctl_result       => fun K =>
+                              match K with
+                              | KCTL_TRAP => ty_exception_type
+                              | KCTL_MRET => ty_unit
+                              end
+      end.
 
-  Definition 𝑼_unfold (U : 𝑼) : 𝑼𝑻 U -> { K : 𝑼𝑲 U & Val (𝑼𝑲_Ty U K) } :=
-    match U as u return (𝑼𝑻 u -> {K : 𝑼𝑲 u & Val (𝑼𝑲_Ty u K)}) with
-    | ast              => fun Kv =>
-                            match Kv with
-                            | RTYPE rs2 rs1 rd op   => existT KRTYPE (tt , rs2 , rs1 , rd , op)
-                            | ITYPE imm rs1 rd op   => existT KITYPE (tt , imm , rs1 , rd , op)
-                            | UTYPE imm rd op       => existT KUTYPE (tt , imm , rd , op)
-                            | BTYPE imm rs2 rs1 op  => existT KBTYPE (tt , imm , rs2 , rs1 , op)
-                            | RISCV_JAL imm rd      => existT KRISCV_JAL (tt , imm , rd)
-                            | RISCV_JALR imm rs1 rd => existT KRISCV_JALR (tt , imm , rs1 , rd)
-                            | LOAD imm rs1 rd       => existT KLOAD (tt , imm , rs1 , rd)
-                            | STORE imm rs2 rs1     => existT KSTORE (tt , imm , rs2 , rs1)
-                            | ECALL                 => existT KECALL tt
-                            | MRET                  => existT KMRET tt
-                            | CSR csr rs1 rd op     => existT KCSR (tt , csr , rs1 , rd , op)
-                            end
-    | access_type      => fun Kv =>
-                            match Kv with
-                            | Read      => existT KRead tt
-                            | Write     => existT KWrite tt
-                            | ReadWrite => existT KReadWrite tt
-                            | Execute   => existT KExecute tt
-                            end
-    | exception_type   => fun Kv =>
-                            match Kv with
-                            | E_Fetch_Access_Fault => existT KE_Fetch_Access_Fault tt
-                            | E_Load_Access_Fault  => existT KE_Load_Access_Fault tt
-                            | E_SAMO_Access_Fault  => existT KE_SAMO_Access_Fault tt
-                            | E_U_EnvCall          => existT KE_U_EnvCall tt
-                            | E_M_EnvCall          => existT KE_M_EnvCall tt
-                            | E_Illegal_Instr      => existT KE_Illegal_Instr tt
-                            end
-    | memory_op_result => fun Kv =>
-                            match Kv with
-                            | MemValue v     => existT KMemValue v
-                            | MemException e => existT KMemException e
-                            end
-    | fetch_result     => fun Kv =>
-                            match Kv with
-                            | F_Base v    => existT KF_Base v
-                            | F_Error e v => existT KF_Error (e , v)
-                            end
-    | ctl_result       => fun Kv =>
-                            match Kv with
-                            | CTL_TRAP e => existT KCTL_TRAP e
-                            | CTL_MRET   => existT KCTL_MRET tt
-                            end
-    end.
+    Definition 𝑼_unfold (U : 𝑼) : 𝑼𝑻 U -> { K : 𝑼𝑲 U & Val (𝑼𝑲_Ty U K) } :=
+      match U as u return (𝑼𝑻 u -> {K : 𝑼𝑲 u & Val (𝑼𝑲_Ty u K)}) with
+      | ast              => fun Kv =>
+                              match Kv with
+                              | RTYPE rs2 rs1 rd op   => existT KRTYPE (tt , rs2 , rs1 , rd , op)
+                              | ITYPE imm rs1 rd op   => existT KITYPE (tt , imm , rs1 , rd , op)
+                              | UTYPE imm rd op       => existT KUTYPE (tt , imm , rd , op)
+                              | BTYPE imm rs2 rs1 op  => existT KBTYPE (tt , imm , rs2 , rs1 , op)
+                              | RISCV_JAL imm rd      => existT KRISCV_JAL (tt , imm , rd)
+                              | RISCV_JALR imm rs1 rd => existT KRISCV_JALR (tt , imm , rs1 , rd)
+                              | LOAD imm rs1 rd       => existT KLOAD (tt , imm , rs1 , rd)
+                              | STORE imm rs2 rs1     => existT KSTORE (tt , imm , rs2 , rs1)
+                              | ECALL                 => existT KECALL tt
+                              | MRET                  => existT KMRET tt
+                              | CSR csr rs1 rd op     => existT KCSR (tt , csr , rs1 , rd , op)
+                              end
+      | access_type      => fun Kv =>
+                              match Kv with
+                              | Read      => existT KRead tt
+                              | Write     => existT KWrite tt
+                              | ReadWrite => existT KReadWrite tt
+                              | Execute   => existT KExecute tt
+                              end
+      | exception_type   => fun Kv =>
+                              match Kv with
+                              | E_Fetch_Access_Fault => existT KE_Fetch_Access_Fault tt
+                              | E_Load_Access_Fault  => existT KE_Load_Access_Fault tt
+                              | E_SAMO_Access_Fault  => existT KE_SAMO_Access_Fault tt
+                              | E_U_EnvCall          => existT KE_U_EnvCall tt
+                              | E_M_EnvCall          => existT KE_M_EnvCall tt
+                              | E_Illegal_Instr      => existT KE_Illegal_Instr tt
+                              end
+      | memory_op_result => fun Kv =>
+                              match Kv with
+                              | MemValue v     => existT KMemValue v
+                              | MemException e => existT KMemException e
+                              end
+      | fetch_result     => fun Kv =>
+                              match Kv with
+                              | F_Base v    => existT KF_Base v
+                              | F_Error e v => existT KF_Error (e , v)
+                              end
+      | ctl_result       => fun Kv =>
+                              match Kv with
+                              | CTL_TRAP e => existT KCTL_TRAP e
+                              | CTL_MRET   => existT KCTL_MRET tt
+                              end
+      end.
 
-  Definition 𝑼_fold (U : 𝑼) : { K : 𝑼𝑲 U & Val (𝑼𝑲_Ty U K) } -> 𝑼𝑻 U :=
-    match U with
-    | ast              => fun Kv =>
-                            match Kv with
-                            | existT KRTYPE (tt , rs2 , rs1 , rd , op)  => RTYPE rs2 rs1 rd op
-                            | existT KITYPE (tt , imm , rs1 , rd , op)  => ITYPE imm rs1 rd op
-                            | existT KUTYPE (tt , imm , rd , op)        => UTYPE imm rd op
-                            | existT KBTYPE (tt , imm , rs2 , rs1 , op) => BTYPE imm rs2 rs1 op
-                            | existT KRISCV_JAL (tt , imm , rd)         => RISCV_JAL imm rd
-                            | existT KRISCV_JALR (tt , imm , rs1 , rd)  => RISCV_JALR imm rs1 rd
-                            | existT KLOAD (tt , imm , rs1 , rd)        => LOAD imm rs1 rd
-                            | existT KSTORE (tt , imm , rs2 , rs1)      => STORE imm rs2 rs1
-                            | existT KECALL tt                          => ECALL
-                            | existT KMRET tt                           => MRET
-                            | existT KCSR (tt , csr , rs1 , rd , op)    => CSR csr rs1 rd op
-                            end
-    | access_type      => fun Kv =>
-                            match Kv with
-                            | existT KRead tt      => Read
-                            | existT KWrite tt     => Write
-                            | existT KReadWrite tt => ReadWrite
-                            | existT KExecute tt   => Execute
-                            end
-    | exception_type   => fun Kv =>
-                            match Kv with
-                            | existT KE_Fetch_Access_Fault tt => E_Fetch_Access_Fault
-                            | existT KE_Load_Access_Fault tt  => E_Load_Access_Fault
-                            | existT KE_SAMO_Access_Fault tt  => E_SAMO_Access_Fault
-                            | existT KE_U_EnvCall tt          => E_U_EnvCall
-                            | existT KE_M_EnvCall tt          => E_M_EnvCall
-                            | existT KE_Illegal_Instr tt      => E_Illegal_Instr
-                            end
-    | memory_op_result => fun Kv =>
-                            match Kv with
-                            | existT KMemValue v     => MemValue v
-                            | existT KMemException e => MemException e
-                            end
-    | fetch_result     => fun Kv =>
-                            match Kv with
-                            | existT KF_Base v        => F_Base v
-                            | existT KF_Error (e , v) => F_Error e v
-                            end
-    | ctl_result       => fun Kv =>
-                            match Kv with
-                            | existT KCTL_TRAP e  => CTL_TRAP e
-                            | existT KCTL_MRET tt => CTL_MRET
-                            end
-    end.
+    Definition 𝑼_fold (U : 𝑼) : { K : 𝑼𝑲 U & Val (𝑼𝑲_Ty U K) } -> 𝑼𝑻 U :=
+      match U with
+      | ast              => fun Kv =>
+                              match Kv with
+                              | existT KRTYPE (tt , rs2 , rs1 , rd , op)  => RTYPE rs2 rs1 rd op
+                              | existT KITYPE (tt , imm , rs1 , rd , op)  => ITYPE imm rs1 rd op
+                              | existT KUTYPE (tt , imm , rd , op)        => UTYPE imm rd op
+                              | existT KBTYPE (tt , imm , rs2 , rs1 , op) => BTYPE imm rs2 rs1 op
+                              | existT KRISCV_JAL (tt , imm , rd)         => RISCV_JAL imm rd
+                              | existT KRISCV_JALR (tt , imm , rs1 , rd)  => RISCV_JALR imm rs1 rd
+                              | existT KLOAD (tt , imm , rs1 , rd)        => LOAD imm rs1 rd
+                              | existT KSTORE (tt , imm , rs2 , rs1)      => STORE imm rs2 rs1
+                              | existT KECALL tt                          => ECALL
+                              | existT KMRET tt                           => MRET
+                              | existT KCSR (tt , csr , rs1 , rd , op)    => CSR csr rs1 rd op
+                              end
+      | access_type      => fun Kv =>
+                              match Kv with
+                              | existT KRead tt      => Read
+                              | existT KWrite tt     => Write
+                              | existT KReadWrite tt => ReadWrite
+                              | existT KExecute tt   => Execute
+                              end
+      | exception_type   => fun Kv =>
+                              match Kv with
+                              | existT KE_Fetch_Access_Fault tt => E_Fetch_Access_Fault
+                              | existT KE_Load_Access_Fault tt  => E_Load_Access_Fault
+                              | existT KE_SAMO_Access_Fault tt  => E_SAMO_Access_Fault
+                              | existT KE_U_EnvCall tt          => E_U_EnvCall
+                              | existT KE_M_EnvCall tt          => E_M_EnvCall
+                              | existT KE_Illegal_Instr tt      => E_Illegal_Instr
+                              end
+      | memory_op_result => fun Kv =>
+                              match Kv with
+                              | existT KMemValue v     => MemValue v
+                              | existT KMemException e => MemException e
+                              end
+      | fetch_result     => fun Kv =>
+                              match Kv with
+                              | existT KF_Base v        => F_Base v
+                              | existT KF_Error (e , v) => F_Error e v
+                              end
+      | ctl_result       => fun Kv =>
+                              match Kv with
+                              | existT KCTL_TRAP e  => CTL_TRAP e
+                              | existT KCTL_MRET tt => CTL_MRET
+                              end
+      end.
 
-  Lemma 𝑼_fold_unfold : forall (U : 𝑼) (Kv: 𝑼𝑻 U),
-      𝑼_fold U (𝑼_unfold U Kv) = Kv.
-  Proof. now intros [] []. Qed.
-  Lemma 𝑼_unfold_fold : forall (U : 𝑼) (Kv: { K : 𝑼𝑲 U & Val (𝑼𝑲_Ty U K) }),
-      𝑼_unfold U (𝑼_fold U Kv) = Kv.
-  Proof.
-    intros [] [[] x]; cbn in x;
-      repeat match goal with
-             | x: unit     |- _ => destruct x
-             | x: prod _ _ |- _ => destruct x
-             end; auto.
-  Qed.
+    Lemma 𝑼_fold_unfold : forall (U : 𝑼) (Kv: 𝑼𝑻 U),
+        𝑼_fold U (𝑼_unfold U Kv) = Kv.
+    Proof. now intros [] []. Qed.
+    Lemma 𝑼_unfold_fold : forall (U : 𝑼) (Kv: { K : 𝑼𝑲 U & Val (𝑼𝑲_Ty U K) }),
+        𝑼_unfold U (𝑼_fold U Kv) = Kv.
+    Proof.
+      intros [] [[] x]; cbn in x;
+        repeat match goal with
+               | x: unit     |- _ => destruct x
+               | x: prod _ _ |- _ => destruct x
+               end; auto.
+    Qed.
 
-  (** Records **)
-  Definition 𝑹𝑭  : Set := string.
+    (** Records **)
+    Definition 𝑹𝑭  : Set := string.
 
-  Definition 𝑹𝑭_Ty (R : 𝑹) : NCtx 𝑹𝑭 Ty :=
-    match R with
-    | rpmpcfg_ent => [ "L" ∷ ty_bool;
-                       "A" ∷ ty_pmpaddrmatchtype;
-                       "X" ∷ ty_bool;
-                       "W" ∷ ty_bool;
-                       "R" ∷ ty_bool
-                     ]
-    | rmstatus    => ["MPP" ∷ ty_privilege
-                    ]
-    end.
+    Definition 𝑹𝑭_Ty (R : 𝑹) : NCtx 𝑹𝑭 Ty :=
+      match R with
+      | rpmpcfg_ent => [ "L" ∷ ty_bool;
+                         "A" ∷ ty_pmpaddrmatchtype;
+                         "X" ∷ ty_bool;
+                         "W" ∷ ty_bool;
+                         "R" ∷ ty_bool
+        ]
+      | rmstatus    => ["MPP" ∷ ty_privilege
+        ]
+      end.
 
-  Equations 𝑹_fold (R : 𝑹) : NamedEnv Val (𝑹𝑭_Ty R) -> 𝑹𝑻 R :=
-  | rpmpcfg_ent | [l;a;x;w;r]%env := MkPmpcfg_ent l a x w r
-  | rmstatus    | [mpp]%env       := MkMstatus mpp.
+    Equations 𝑹_fold (R : 𝑹) : NamedEnv Val (𝑹𝑭_Ty R) -> 𝑹𝑻 R :=
+    | rpmpcfg_ent | [l;a;x;w;r]%env := MkPmpcfg_ent l a x w r
+    | rmstatus    | [mpp]%env       := MkMstatus mpp.
 
-  Equations 𝑹_unfold (R : 𝑹) : 𝑹𝑻 R -> NamedEnv Val (𝑹𝑭_Ty R) :=
-  | rpmpcfg_ent | p => [kv (_ ∷ ty_bool             ; L p);
-                           (_ ∷ ty_pmpaddrmatchtype ; A p);
-                           (_ ∷ ty_bool             ; X p);
-                           (_ ∷ ty_bool             ; W p);
-                           (_ ∷ ty_bool             ; R p) ];
-  | rmstatus    | m => [kv ("MPP" ∷ ty_privilege; MPP m) ].
+    Equations 𝑹_unfold (R : 𝑹) : 𝑹𝑻 R -> NamedEnv Val (𝑹𝑭_Ty R) :=
+    | rpmpcfg_ent | p => [kv (_ ∷ ty_bool             ; L p);
+                          (_ ∷ ty_pmpaddrmatchtype ; A p);
+                          (_ ∷ ty_bool             ; X p);
+                          (_ ∷ ty_bool             ; W p);
+                          (_ ∷ ty_bool             ; R p) ];
+    | rmstatus    | m => [kv ("MPP" ∷ ty_privilege; MPP m) ].
 
-  Lemma 𝑹_fold_unfold : forall (R : 𝑹) (Kv: 𝑹𝑻 R),
-      𝑹_fold R (𝑹_unfold R Kv) = Kv.
-  Proof. now intros [] []. Qed.
-  Lemma 𝑹_unfold_fold : forall (R : 𝑹) (Kv: NamedEnv Val (𝑹𝑭_Ty R)),
-      𝑹_unfold R (𝑹_fold R Kv) = Kv.
-  Proof. intros []; now apply env.Forall_forall. Qed.
+    Lemma 𝑹_fold_unfold : forall (R : 𝑹) (Kv: 𝑹𝑻 R),
+        𝑹_fold R (𝑹_unfold R Kv) = Kv.
+    Proof. now intros [] []. Qed.
+    Lemma 𝑹_unfold_fold : forall (R : 𝑹) (Kv: NamedEnv Val (𝑹𝑭_Ty R)),
+        𝑹_unfold R (𝑹_fold R Kv) = Kv.
+    Proof. intros []; now apply env.Forall_forall. Qed.
 
-End TypeDefKit.
+  End TypeDefKit.
 
-Section RegDeclKit.
+  Section RegDeclKit.
 
-  Inductive Reg : Ty -> Set :=
-  | pc            : Reg ty_xlenbits
-  | nextpc        : Reg ty_xlenbits
-  | mstatus       : Reg ty_mstatus
-  | mtvec         : Reg ty_xlenbits
-  | mcause        : Reg ty_exc_code
-  | mepc          : Reg ty_xlenbits
-  | cur_privilege : Reg ty_privilege
-  | x1            : Reg ty_xlenbits
-  | x2            : Reg ty_xlenbits
-  | x3            : Reg ty_xlenbits
-  | x4            : Reg ty_xlenbits
-  | x5            : Reg ty_xlenbits
-  | x6            : Reg ty_xlenbits
-  | x7            : Reg ty_xlenbits
-  | pmp0cfg       : Reg ty_pmpcfg_ent
-  | pmp1cfg       : Reg ty_pmpcfg_ent
-  | pmpaddr0      : Reg ty_xlenbits
-  | pmpaddr1      : Reg ty_xlenbits
-  .
+    Inductive Reg : Ty -> Set :=
+    | pc            : Reg ty_xlenbits
+    | nextpc        : Reg ty_xlenbits
+    | mstatus       : Reg ty_mstatus
+    | mtvec         : Reg ty_xlenbits
+    | mcause        : Reg ty_exc_code
+    | mepc          : Reg ty_xlenbits
+    | cur_privilege : Reg ty_privilege
+    | x1            : Reg ty_xlenbits
+    | x2            : Reg ty_xlenbits
+    | x3            : Reg ty_xlenbits
+    | x4            : Reg ty_xlenbits
+    | x5            : Reg ty_xlenbits
+    | x6            : Reg ty_xlenbits
+    | x7            : Reg ty_xlenbits
+    | pmp0cfg       : Reg ty_pmpcfg_ent
+    | pmp1cfg       : Reg ty_pmpcfg_ent
+    | pmpaddr0      : Reg ty_xlenbits
+    | pmpaddr1      : Reg ty_xlenbits
+    .
 
-  Import bv.notations.
-  Definition reg_convert (idx : RegIdx) : option (Reg ty_xlenbits) :=
-    match bv.to_bitstring idx with
-    | 000 => None
-    | 001 => Some x1
-    | 010 => Some x2
-    | 011 => Some x3
-    | 100 => Some x4
-    | 101 => Some x5
-    | 110 => Some x6
-    | 111 => Some x7
-    end.
+    Import bv.notations.
+    Definition reg_convert (idx : RegIdx) : option (Reg ty_xlenbits) :=
+      match bv.to_bitstring idx with
+      | 000 => None
+      | 001 => Some x1
+      | 010 => Some x2
+      | 011 => Some x3
+      | 100 => Some x4
+      | 101 => Some x5
+      | 110 => Some x6
+      | 111 => Some x7
+      end.
 
-  Section TransparentObligations.
-    Local Set Transparent Obligations.
-    Derive Signature NoConfusion NoConfusionHom EqDec for Reg.
-  End TransparentObligations.
+    Section TransparentObligations.
+      Local Set Transparent Obligations.
+      Derive Signature NoConfusion NoConfusionHom EqDec for Reg.
+    End TransparentObligations.
 
-  Definition 𝑹𝑬𝑮 : Ty -> Set := Reg.
-  Instance 𝑹𝑬𝑮_eq_dec : EqDec (sigT Reg) :=
-    sigma_eqdec _ _.
+    Definition 𝑹𝑬𝑮 : Ty -> Set := Reg.
+    Instance 𝑹𝑬𝑮_eq_dec : EqDec (sigT Reg) :=
+      sigma_eqdec _ _.
 
-  Local Obligation Tactic :=
-    finite_from_eqdec.
+    Local Obligation Tactic :=
+      finite_from_eqdec.
 
-  Program Instance 𝑹𝑬𝑮_finite : Finite (sigT Reg) :=
-    {| enum :=
-       [ existT _ pc;
-         existT _ nextpc;
-         existT _ mstatus;
-         existT _ mtvec;
-         existT _ mcause;
-         existT _ mepc;
-         existT _ cur_privilege;
-         existT _ x1;
-         existT _ x2;
-         existT _ x3;
-         existT _ x4;
-         existT _ x5;
-         existT _ x6;
-         existT _ x7;
-         existT _ pmp0cfg;
-         existT _ pmp1cfg;
-         existT _ pmpaddr0;
-         existT _ pmpaddr1
-       ]%list
-    |}.
+    Program Instance 𝑹𝑬𝑮_finite : Finite (sigT Reg) :=
+      {| enum :=
+        [ existT _ pc;
+          existT _ nextpc;
+          existT _ mstatus;
+          existT _ mtvec;
+          existT _ mcause;
+          existT _ mepc;
+          existT _ cur_privilege;
+          existT _ x1;
+          existT _ x2;
+          existT _ x3;
+          existT _ x4;
+          existT _ x5;
+          existT _ x6;
+          existT _ x7;
+          existT _ pmp0cfg;
+          existT _ pmp1cfg;
+          existT _ pmpaddr0;
+          existT _ pmpaddr1
+        ]%list
+      |}.
 
-End RegDeclKit.
+  End RegDeclKit.
 
-Include BaseMixin.
+  Include BaseMixin.
 
 End RiscvPmpBase.
